ems/SimGlobalIndex2Explicit1.v
@@ -18,12 +18,17 @@ Set Implicit Arguments.
 
 Section SIM.
 
+  Variable E: Type -> Type.
+
   Inductive _simg_aux
-            (simg_aux: forall R0 R1 (RR: Ord.t -> Ord.t -> R0 -> R1 -> Prop), Ord.t -> Ord.t -> (itree eventE R0) -> (itree eventE R1) -> Prop)
-            {R0 R1} (RR: Ord.t -> Ord.t -> R0 -> R1 -> Prop) (f_src f_tgt: Ord.t): (itree eventE R0) -> (itree eventE R1) -> Prop :=
+            (simg_aux: forall R0 R1 (RR: Ord.t -> Ord.t -> R0 -> R1 -> Prop), Ord.t -> Ord.t -> (itree (E +' eventE) R0) -> (itree (E +' eventE) R1) -> Prop)
+            {R0 R1} (RR: Ord.t -> Ord.t -> R0 -> R1 -> Prop) (f_src f_tgt: Ord.t): (itree (E +' eventE) R0) -> (itree (E +' eventE) R1) -> Prop :=
   | simg_aux_ret
+      f_src' f_tgt'
+      (LE: (f_src' <= f_src)%ord)
+      (LE: (f_tgt' <= f_tgt)%ord)
       r_src r_tgt
-      (SIM: RR f_src f_tgt r_src r_tgt)
+      (SIM: RR f_src' f_tgt' r_src r_tgt)
     :
     _simg_aux simg_aux RR f_src f_tgt (Ret r_src) (Ret r_tgt)
   | simg_aux_syscall
@@ -80,15 +85,25 @@ Section SIM.
       (TGT: (f_tgt0 < f_tgt)%ord)
     :
     _simg_aux simg_aux RR f_src f_tgt itr_src itr_tgt
+
+  | simg_aux_event
+      X (e: E X) ktr_src0 ktr_tgt0
+      f_src0 f_tgt0
+      (SIM: forall x_src x_tgt (EQ: x_src = x_tgt), @_simg_aux simg_aux _ _ RR f_src0 f_tgt0 (ktr_src0 x_src) (ktr_tgt0 x_tgt))
+    :
+    _simg_aux simg_aux RR f_src f_tgt (trigger e >>= ktr_src0) (trigger e >>= ktr_tgt0)
   .
 
-  Lemma _simg_aux_ind2 (r: forall R0 R1 (RR: Ord.t -> Ord.t -> R0 -> R1 -> Prop), Ord.t -> Ord.t -> (itree eventE R0) -> (itree eventE R1) -> Prop)
+  Lemma _simg_aux_ind2 (r: forall R0 R1 (RR: Ord.t -> Ord.t -> R0 -> R1 -> Prop), Ord.t -> Ord.t -> (itree (E +' eventE) R0) -> (itree (E +' eventE) R1) -> Prop)
         R0 R1 (RR: Ord.t -> Ord.t -> R0 -> R1 -> Prop)
-        (P: Ord.t -> Ord.t -> (itree eventE R0) -> (itree eventE R1) -> Prop)
+        (P: Ord.t -> Ord.t -> (itree (E +' eventE) R0) -> (itree (E +' eventE) R1) -> Prop)
         (RET: forall
             f_src f_tgt
+            f_src' f_tgt'
+            (LE: (f_src' <= f_src)%ord)
+            (LE: (f_tgt' <= f_tgt)%ord)
             r_src r_tgt
-            (SIM: RR f_src f_tgt r_src r_tgt),
+            (SIM: RR f_src' f_tgt' r_src r_tgt),
             P f_src f_tgt (Ret r_src) (Ret r_tgt))
         (SYSCALL: forall
             f_src f_tgt
@@ -148,6 +163,12 @@ Section SIM.
             (SRC: (f_src0 < f_src)%ord)
             (TGT: (f_tgt0 < f_tgt)%ord),
             P f_src f_tgt itr_src itr_tgt)
+        (EVENT: forall
+            f_src f_tgt
+            f_src0 f_tgt0
+            X (e: E X) ktr_src0 ktr_tgt0
+            (SIM: forall x_src x_tgt (EQ: x_src = x_tgt), (<<SIM: _simg_aux r RR f_src0 f_tgt0 (ktr_src0 x_src) (ktr_tgt0 x_tgt)>>) /\ (<<IH: P f_src0 f_tgt0 (ktr_src0 x_src) (ktr_tgt0 x_tgt)>>)),
+            P f_src f_tgt (trigger e >>= ktr_src0) (trigger e >>= ktr_tgt0))
     :
     forall f_src f_tgt itr_src itr_tgt
       (SIM: _simg_aux r RR f_src f_tgt itr_src itr_tgt),
@@ -163,9 +184,10 @@ Section SIM.
     { eapply TAKEL; eauto. }
     { eapply TAKER; eauto. des. esplits; eauto. }
     { eapply PROGRESS; eauto. }
+    { eapply EVENT; eauto. i. split; eauto. }
   Qed.
 
-  Definition simg_aux: forall R0 R1 (RR: Ord.t -> Ord.t -> R0 -> R1 -> Prop), Ord.t -> Ord.t -> (itree eventE R0) -> (itree eventE R1) -> Prop := paco7 _simg_aux bot7.
+  Definition simg_aux: forall R0 R1 (RR: Ord.t -> Ord.t -> R0 -> R1 -> Prop), Ord.t -> Ord.t -> (itree (E +' eventE) R0) -> (itree (E +' eventE) R1) -> Prop := paco7 _simg_aux bot7.
 
   Lemma simg_aux_mon: monotone7 _simg_aux.
   Proof.
@@ -179,17 +201,21 @@ Section SIM.
     { econs 7; eauto. i. spc SIM. des; et. }
     { econs 8; eauto. des. esplits; eauto. }
     { econs 9; eauto. }
+    { econs 10; eauto. i. specialize (SIM x_src x_tgt EQ). des; eauto. }
   Qed.
   Hint Resolve simg_aux_mon: paco.
   Hint Resolve cpn7_wcompat: paco.
 
 
   Variant simg_aux_indC
-          (simg_aux: forall R0 R1 (RR: Ord.t -> Ord.t -> R0 -> R1 -> Prop), Ord.t -> Ord.t -> (itree eventE R0) -> (itree eventE R1) -> Prop)
-          {R0 R1} (RR: Ord.t -> Ord.t -> R0 -> R1 -> Prop) (f_src f_tgt: Ord.t): (itree eventE R0) -> (itree eventE R1) -> Prop :=
+          (simg_aux: forall R0 R1 (RR: Ord.t -> Ord.t -> R0 -> R1 -> Prop), Ord.t -> Ord.t -> (itree (E +' eventE) R0) -> (itree (E +' eventE) R1) -> Prop)
+          {R0 R1} (RR: Ord.t -> Ord.t -> R0 -> R1 -> Prop) (f_src f_tgt: Ord.t): (itree (E +' eventE) R0) -> (itree (E +' eventE) R1) -> Prop :=
     | simg_aux_indC_ret
+        f_src' f_tgt'
+        (LE: (f_src' <= f_src)%ord)
+        (LE: (f_tgt' <= f_tgt)%ord)
         r_src r_tgt
-        (SIM: RR f_src f_tgt r_src r_tgt)
+        (SIM: RR f_src' f_tgt' r_src r_tgt)
       :
       simg_aux_indC simg_aux RR f_src f_tgt (Ret r_src) (Ret r_tgt)
     | simg_aux_indC_syscall
@@ -237,6 +263,13 @@ Section SIM.
         (SIM: exists x, simg_aux _ _ RR f_src f_tgt0 itr_src0 (ktr_tgt0 x))
       :
       simg_aux_indC simg_aux RR f_src f_tgt (itr_src0) (trigger (Take X) >>= ktr_tgt0)
+
+    | simg_aux_indC_event
+        f_src0 f_tgt0
+        X (e: E X) ktr_src0 ktr_tgt0
+        (SIM: forall x_src x_tgt (EQ: x_src = x_tgt), simg_aux _ _ RR f_src0 f_tgt0 (ktr_src0 x_src) (ktr_tgt0 x_tgt))
+      :
+      simg_aux_indC simg_aux RR f_src f_tgt (trigger e >>= ktr_src0) (trigger e >>= ktr_tgt0)
   .
 
   Lemma simg_aux_indC_mon: monotone7 simg_aux_indC.
@@ -250,6 +283,7 @@ Section SIM.
     { econs 6; eauto. }
     { econs 7; eauto. }
     { econs 8; eauto. des. esplits; eauto. }
+    { econs 9; eauto. }
   Qed.
   Hint Resolve simg_aux_indC_mon: paco.
 
@@ -267,14 +301,19 @@ Section SIM.
     { econs 6; eauto. i. eapply simg_aux_mon; eauto. i. eapply rclo7_base; eauto. }
     { econs 7; eauto. i. eapply simg_aux_mon; eauto. i. eapply rclo7_base; eauto. }
     { des. econs 8; eauto. esplits. eapply simg_aux_mon; eauto. i. eapply rclo7_base; eauto. }
+    { econs 10; eauto. i. specialize (SIM x_src x_tgt EQ). eapply simg_aux_mon. eauto.
+      i. eapply rclo7_base. auto. }
   Qed.
 
   Lemma simg_aux_ind R0 R1 (RR: Ord.t -> Ord.t -> R0 -> R1 -> Prop)
-        (P: Ord.t -> Ord.t -> (itree eventE R0) -> (itree eventE R1) -> Prop)
+        (P: Ord.t -> Ord.t -> (itree (E +' eventE) R0) -> (itree (E +' eventE) R1) -> Prop)
         (RET: forall
             f_src f_tgt
+            f_src' f_tgt'
+            (LE: (f_src' <= f_src)%ord)
+            (LE: (f_tgt' <= f_tgt)%ord)
             r_src r_tgt
-            (SIM: RR f_src f_tgt r_src r_tgt),
+            (SIM: RR f_src' f_tgt' r_src r_tgt),
             P f_src f_tgt (Ret r_src) (Ret r_tgt))
         (SYSCALL: forall
             f_src0 f_tgt0
@@ -328,6 +367,12 @@ Section SIM.
             (SRC: (f_src0 < f_src)%ord)
             (TGT: (f_tgt0 < f_tgt)%ord),
             P f_src f_tgt itr_src itr_tgt)
+        (EVENT: forall
+            f_src0 f_tgt0
+            f_src f_tgt
+            X (e: E X) ktr_src0 ktr_tgt0
+            (SIM: forall x_src x_tgt (EQ: x_src = x_tgt), (<<SIMG: simg_aux RR f_src0 f_tgt0 (ktr_src0 x_src) (ktr_tgt0 x_tgt)>>) /\ (<<IH: P f_src0 f_tgt0 (ktr_src0 x_src) (ktr_tgt0 x_tgt)>>)),
+            P f_src f_tgt (trigger e >>= ktr_src0) (trigger e >>= ktr_tgt0))
     :
     forall f_src f_tgt itr_src itr_tgt
       (SIM: simg_aux RR f_src f_tgt itr_src itr_tgt),
@@ -343,6 +388,7 @@ Section SIM.
     { eapply TAKEL; eauto. i. hexploit SIM; eauto. i. des. esplits; eauto. pfold. auto. }
     { eapply TAKER; eauto. des. esplits; eauto. pfold. auto. }
     { eapply PROGRESS; eauto. pclearbot. auto. }
+    { eapply EVENT; eauto. i. hexploit SIM; eauto. i. des. split; eauto. pfold. auto. }
   Qed.
 
   Hint Constructors _simg_aux.
@@ -361,10 +407,12 @@ Hint Resolve cpn7_wcompat: paco.
 
 Section PROOF.
 
+  Variable E: Type -> Type.
+
   Lemma simg_implies_simg_aux
         R0 R1 (RR: Ord.t -> Ord.t -> R0 -> R1 -> Prop)
-        (itr_src: itree eventE R0)
-        (itr_tgt: itree eventE R1)
+        (itr_src: itree (E +' eventE) R0)
+        (itr_tgt: itree (E +' eventE) R1)
         (f_src f_tgt: Ord.t)
         (SIM: simg RR f_src f_tgt (itr_src) (itr_tgt))
     :
@@ -384,6 +432,10 @@ Section PROOF.
     { guclo simg_aux_indC_spec. econs 7. i. specialize (SIM x). des. eauto. }
     { des. guclo simg_aux_indC_spec. }
     { gstep. econs 9; eauto. gfinal. left; eauto. }
+    { gstep. econs 10. i. specialize (SIM _ _ EQ).
+      instantiate (2:= Ord.S f_src0). instantiate (1:= Ord.S f_tgt0).
+      econs 9. gfinal. left. eauto. 1,2: apply Ord.S_lt.
+    }
   Qed.
 
 End PROOF.
@@ -392,14 +444,18 @@ End PROOF.
 
 Section GEN.
 
+  Variable E: Type -> Type.
   Variable wf: WF.
 
   Inductive gen_exp
-            {R0 R1} (RR: Ord.t -> Ord.t -> R0 -> R1 -> Prop) (f_src f_tgt: Ord.t): (wf.(T)) -> (itree eventE R0) -> (wf.(T)) -> (itree eventE R1) -> Prop :=
+            {R0 R1} (RR: Ord.t -> Ord.t -> R0 -> R1 -> Prop) (f_src f_tgt: Ord.t): (wf.(T)) -> (itree (E +' eventE) R0) -> (wf.(T)) -> (itree (E +' eventE) R1) -> Prop :=
   | gen_exp_ret
       r_src r_tgt
+      f_src' f_tgt'
+      (LE: (f_src' <= f_src)%ord)
+      (LE: (f_tgt' <= f_tgt)%ord)
       g_src g_tgt
-      (GEN: RR f_src f_tgt r_src r_tgt)
+      (GEN: RR f_src' f_tgt' r_src r_tgt)
     :
     gen_exp RR f_src f_tgt (g_src) (Ret r_src) (g_tgt) (Ret r_tgt)
   | gen_exp_syscall
@@ -475,12 +531,23 @@ Section GEN.
       (TGT: (f_tgt0 < f_tgt)%ord)
     :
     gen_exp RR f_src f_tgt (g_src) (itr_src) (g_tgt) (itr_tgt)
+
+  | gen_exp_event
+      X (e: E X) ktr_src0 ktr_tgt0
+      f_src0 f_tgt0
+      g_src g_tgt g_src0 g_tgt0
+      (LTS: wf.(lt) g_src0 g_src)
+      (LTT: wf.(lt) g_tgt0 g_tgt)
+      (GEN: forall x_src x_tgt (EQ: x_src = x_tgt),
+          gen_exp RR f_src0 f_tgt0 (g_src0) (ktr_src0 x_src) (g_tgt0) (ktr_tgt0 x_tgt))
+    :
+    gen_exp RR f_src f_tgt (g_src) (trigger e >>= ktr_src0) (g_tgt) (trigger e >>= ktr_tgt0)
   .
 
   Lemma gen_exp_leL
         R0 R1 (RR: Ord.t -> Ord.t -> R0 -> R1 -> Prop)
-        (itr_src: itree eventE R0)
-        (itr_tgt: itree eventE R1)
+        (itr_src: itree (E +' eventE) R0)
+        (itr_tgt: itree (E +' eventE) R1)
         (f_src f_tgt: Ord.t)
         gs0 gs1 gt
         (LE: wf.(le) gs0 gs1)
@@ -491,7 +558,7 @@ Section GEN.
     destruct LE.
     { clarify. }
     rename H into LT. generalize dependent gs1. induction GEN; i.
-    { econs 1. eauto. }
+    { econs 1; eauto. }
     { econs 2.
       3:{ i. specialize (H _ _ EQ _ LTS). eauto. }
       all: auto.
@@ -512,12 +579,16 @@ Section GEN.
     }
     { econs 8. 2: eauto. auto. }
     { econs 9. eauto. all: auto. }
+    { econs 10.
+      3:{ i. specialize (H _ _ EQ _ LTS). eauto. }
+      all: auto.
+    }
   Qed.
 
   Lemma gen_exp_leR
         R0 R1 (RR: Ord.t -> Ord.t -> R0 -> R1 -> Prop)
-        (itr_src: itree eventE R0)
-        (itr_tgt: itree eventE R1)
+        (itr_src: itree (E +' eventE) R0)
+        (itr_tgt: itree (E +' eventE) R1)
         (f_src f_tgt: Ord.t)
         gs gt0 gt1
         (LE: wf.(le) gt0 gt1)
@@ -528,7 +599,7 @@ Section GEN.
     destruct LE.
     { clarify. }
     rename H into LT. generalize dependent gt1. induction GEN; i.
-    { econs 1. eauto. }
+    { econs 1; eauto. }
     { econs 2.
       3:{ i. specialize (H _ _ EQ _ LTT). eauto. }
       all: auto.
@@ -549,6 +620,10 @@ Section GEN.
       auto.
     }
     { econs 9. eauto. all: auto. }
+    { econs 10.
+      3:{ i. specialize (H _ _ EQ _ LTT). eauto. }
+      all: auto.
+    }
   Qed.
 
 End GEN.
@@ -557,21 +632,22 @@ Global Hint Constructors gen_exp.
 
 Section PROOF.
 
+  Variable E: Type -> Type.
+
   Lemma simg_aux_gen_exp
         R0 R1 (RR: Ord.t -> Ord.t -> R0 -> R1 -> Prop)
-        (itr_src: itree eventE R0)
-        (itr_tgt: itree eventE R1)
+        (itr_src: itree (E +' eventE) R0)
+        (itr_tgt: itree (E +' eventE) R1)
         (f_src f_tgt: Ord.t)
         (SIM: simg_aux RR f_src f_tgt (itr_src) (itr_tgt))
     :
-    exists gs gt, gen_exp (@ord_tree_WF ((itree eventE R0) * (itree eventE R1)))
+    exists gs gt, gen_exp (@ord_tree_WF ((itree (E +' eventE) R0) * (itree (E +' eventE) R1)))
                      RR f_src f_tgt gs itr_src gt itr_tgt.
   Proof.
-    set (A:= ((itree eventE R0) * (itree eventE R1))%type). move A before RR.
-    set (def:= (@ITree.spin eventE R0, @ITree.spin eventE R1)). move def before A.
-    (* exists (@ord_tree_WF A). *)
+    set (A:= ((itree (E +' eventE) R0) * (itree (E +' eventE) R1))%type). move A before RR.
+    set (def:= (@ITree.spin (E +' eventE) R0, @ITree.spin (E +' eventE) R1)). move def before A.
     induction SIM using simg_aux_ind.
-    { exists (ord_tree_base A), (ord_tree_base A). econs 1. auto. }
+    { exists (ord_tree_base A), (ord_tree_base A). econs 1; eauto. }
     { hexploit ord_tree_join.
       { instantiate (2:= A).
         instantiate (2:= (fun '(i_s, i_t) =>
@@ -675,6 +751,38 @@ Section PROOF.
       econs 8. 2: eauto. replace gt with (Succ def); ss.
     }
     { exists (ord_tree_base A), (ord_tree_base A). econs 9; eauto. }
+    { hexploit ord_tree_join.
+      { instantiate (2:= A).
+        instantiate (2:= (fun '(i_s, i_t) =>
+                            exists gs gt, gen_exp (@ord_tree_WF A) RR f_src0 f_tgt0 gs i_s gt i_t)).
+        instantiate (1:= fun '(i_s, i_t) o =>
+                           exists gt, gen_exp (@ord_tree_WF A) RR f_src0 f_tgt0 o i_s gt i_t).
+        i. ss. des_ifs.
+      }
+      intros JOIN1. des. rename o1 into gsT.
+      set (Succ1 := (fun _: A => gsT)). exists (ord_tree_cons Succ1).
+      hexploit ord_tree_join.
+      { instantiate (2:= A).
+        instantiate (2:= (fun '(i_s, i_t) =>
+                            exists gt, gen_exp (@ord_tree_WF A) RR f_src0 f_tgt0 gsT i_s gt i_t)).
+        instantiate (1:= fun '(i_s, i_t) o =>
+                           gen_exp (@ord_tree_WF A) RR f_src0 f_tgt0 gsT i_s o i_t).
+        i. ss. des_ifs.
+      }
+      intros JOIN2. des. rename o1 into gtT.
+      set (Succ2 := (fun _: A => gtT)). exists (ord_tree_cons Succ2).
+      eapply gen_exp_event.
+      { instantiate (1:= (Succ1 def)). ss. }
+      { instantiate (1:= (Succ2 def)). ss. }
+      instantiate (1:=f_tgt0). instantiate (1:=f_src0). i. subst Succ1 Succ2. ss.
+      set (itrp := (ktr_src0 x_src, ktr_tgt0 x_tgt)).
+      specialize (JOIN2 itrp). specialize (JOIN1 itrp).
+      subst itrp. ss. specialize (SIM _ _ EQ). des.
+      hexploit JOIN1; clear JOIN1. eauto. i. des.
+      hexploit JOIN2; clear JOIN2.
+      { exists gt0. eapply gen_exp_leL. 2: eauto. right. auto. }
+      i. des. eapply gen_exp_leR. 2: eauto. right. auto.
+    }
   Qed.
 
 End PROOF.
