ems/SimGlobalAlts2Index.v
@@ -17,6 +17,8 @@ Set Implicit Arguments.
 
 Section PROOF.
 
+  Variable E: Type -> Type.
+
   Definition RR_bot {R0 R1} (RRp: Ord.t -> Ord.t -> R0 -> R1 -> Prop) (RR: R0 -> R1 -> Prop) :=
     forall r0 r1, (RR r0 r1) -> (forall o0 o1, RRp o0 o1 r0 r1).
 
@@ -25,20 +27,26 @@ Section PROOF.
           (RR: R0 -> R1 -> Prop)
           (RRp: Ord.t -> Ord.t -> R0 -> R1 -> Prop)
           (TOP: RR_bot RRp RR)
-          (itr_src: itree eventE R0)
-          (itr_tgt: itree eventE R1)
+          (itr_src: itree (E +' eventE) R0)
+          (itr_tgt: itree (E +' eventE) R1)
           (SIM: simg_alt_imp RR itr_src itr_tgt)
     :
     forall (f_src f_tgt: Ord.t), simg RRp f_src f_tgt (itr_src) (itr_tgt).
   Proof.
     ginit. revert_until TOP. gcofix CIH. i.
     revert_until SIM. induction SIM using simg_alt_imp_ind; i.
-    { inv TGT. inv SRC. guclo simg_indC_spec. }
+    { inv TGT. inv SRC. guclo simg_indC_spec. econs 1; eauto. all: refl. }
     { inv TGT. inv SRC. inv ARG. gstep. econs 2. i. specialize (SIM _ _ EQ).
       inv SIM. inv REL. clarify. rewrite ! bind_trigger in *.
       inv H0. apply inj_pair2 in H2. eapply equal_f in H2.
       inv H1. apply inj_pair2 in H0. eapply equal_f in H0.
       rewrite H0, H2 in REL0. gfinal. left. eapply CIH. auto.
+    }
+    { inv TGT. inv SRC. gstep. econs 10. i. specialize (SIM _ _ EQ).
+      inv SIM. inv REL. clarify. rewrite ! bind_trigger in *.
+      inv H0. apply inj_pair2 in H3. eapply equal_f in H3.
+      inv H1. apply inj_pair2 in H4. eapply equal_f in H4.
+      rewrite H3, H4 in REL0. gfinal. left. eapply CIH. auto.
     }
     { guclo simg_indC_spec. inv SIM.
       - econs; auto. des; eauto.
